src/program_logic/ectx_lifting.v
@@ -17,16 +17,17 @@ Local Hint Resolve head_stuck_stuck : core.
 
 Lemma wp_lift_head_step_fupd {s E Φ} e1 :
   to_val e1 = None →
-  (∀ σ1 g1 ns κ κs nt, state_interp σ1 g1 ns (κ ++ κs) nt ={E,∅}=∗ ▷
+  (∀ σ1 g1 ns κ κs nt, state_interp σ1 ns (κ ++ κs) nt -∗ global_state_interp g1 ={E,∅}=∗ ▷
     (⌜head_reducible e1 σ1 g1⌝ ∗
     ∀ e2 σ2 g2 efs, ⌜head_step e1 σ1 g1 κ e2 σ2 g2 efs⌝ ={∅,E}=∗
-      state_interp σ2 g2 (S ns) κs (length efs + nt) ∗
+      state_interp σ2 (S ns) κs (length efs + nt) ∗
+      global_state_interp g2 ∗
       WP e2 @ s; E {{ Φ }} ∗
       [∗ list] ef ∈ efs, WP ef @ s; ⊤ {{ fork_post }}))
   ⊢ WP e1 @ s; E {{ Φ }}.
 Proof.
-  iIntros (?) "H". iApply wp_lift_step_fupd=>//. iIntros (σ1 g1 ns κ κs nt) "Hσ".
-  iMod ("H" with "Hσ") as "H". iModIntro.
+  iIntros (?) "H". iApply wp_lift_step_fupd=>//. iIntros (σ1 g1 ns κ κs nt) "Hσ Hg".
+  iMod ("H" with "Hσ Hg") as "H". iModIntro.
   iNext. iDestruct "H" as "[% H]".
   iSplit; first by destruct s; eauto. iIntros (e2 σ2 g2 efs ?).
   iApply "H"; eauto.
@@ -34,16 +35,17 @@ Qed.
 
 Lemma wp_lift_head_step {s E Φ} e1 :
   to_val e1 = None →
-  (∀ σ1 g1 ns κ κs nt, state_interp σ1 g1 ns (κ ++ κs) nt ={E,∅}=∗
+  (∀ σ1 g1 ns κ κs nt, state_interp σ1 ns (κ ++ κs) nt -∗ global_state_interp g1 ={E,∅}=∗
     ⌜head_reducible e1 σ1 g1⌝ ∗
     ▷ ∀ e2 σ2 g2 efs, ⌜head_step e1 σ1 g1 κ e2 σ2 g2 efs⌝ ={∅,E}=∗
-      state_interp σ2 g2 (S ns) κs (length efs + nt) ∗
+      state_interp σ2 (S ns) κs (length efs + nt) ∗
+      global_state_interp g2 ∗
       WP e2 @ s; E {{ Φ }} ∗
       [∗ list] ef ∈ efs, WP ef @ s; ⊤ {{ fork_post }})
   ⊢ WP e1 @ s; E {{ Φ }}.
 Proof.
-  iIntros (?) "H". iApply wp_lift_head_step_fupd; [done|]. iIntros (??????) "?".
-  iMod ("H" with "[$]") as "[$ H]". iIntros "!> !>" (e2 σ2 g2 efs ?). by iApply "H".
+  iIntros (?) "H". iApply wp_lift_head_step_fupd; [done|]. iIntros (??????) "??".
+  iMod ("H" with "[$] [$]") as "[$ H]". iIntros "!> !>" (e2 σ2 g2 efs ?). by iApply "H".
 Qed.
 
 (*
@@ -88,16 +90,17 @@ Qed.
 
 Lemma wp_lift_atomic_head_step {s E Φ} e1 :
   to_val e1 = None →
-  (∀ σ1 g1 ns κ κs nt, state_interp σ1 g1 ns (κ ++ κs) nt ={E}=∗
+  (∀ σ1 g1 ns κ κs nt, state_interp σ1 ns (κ ++ κs) nt -∗ global_state_interp g1 ={E}=∗
     ⌜head_reducible e1 σ1 g1⌝ ∗
     ▷ ∀ e2 σ2 g2 efs, ⌜head_step e1 σ1 g1 κ e2 σ2 g2 efs⌝ ={E}=∗
-      state_interp σ2 g2 (S ns) κs (length efs + nt) ∗
+      state_interp σ2 (S ns) κs (length efs + nt) ∗
+      global_state_interp g2 ∗
       from_option Φ False (to_val e2) ∗
       [∗ list] ef ∈ efs, WP ef @ s; ⊤ {{ fork_post }})
   ⊢ WP e1 @ s; E {{ Φ }}.
 Proof.
   iIntros (?) "H". iApply wp_lift_atomic_step; eauto.
-  iIntros (σ1 g1 ns κ κs nt) "Hσ1". iMod ("H" with "Hσ1") as "[% H]"; iModIntro.
+  iIntros (σ1 g1 ns κ κs nt) "Hσ1 Hg1". iMod ("H" with "Hσ1 Hg1") as "[% H]"; iModIntro.
   iSplit; first by destruct s; auto. iNext. iIntros (e2 σ2 g2 efs Hstep).
   iApply "H"; eauto.
 Qed.
@@ -121,16 +124,17 @@ Qed.
 
 Lemma wp_lift_atomic_head_step_no_fork {s E Φ} e1 :
   to_val e1 = None →
-  (∀ σ1 g1 ns κ κs nt, state_interp σ1 g1 ns (κ ++ κs) nt ={E}=∗
+  (∀ σ1 g1 ns κ κs nt, state_interp σ1 ns (κ ++ κs) nt -∗ global_state_interp g1 ={E}=∗
     ⌜head_reducible e1 σ1 g1⌝ ∗
     ▷ ∀ e2 σ2 g2 efs, ⌜head_step e1 σ1 g1 κ e2 σ2 g2 efs⌝ ={E}=∗
-      ⌜efs = []⌝ ∗ state_interp σ2 g2 (S ns) κs nt ∗ from_option Φ False (to_val e2))
+      ⌜efs = []⌝ ∗ state_interp σ2 (S ns) κs nt ∗ global_state_interp g2 ∗
+      from_option Φ False (to_val e2))
   ⊢ WP e1 @ s; E {{ Φ }}.
 Proof.
   iIntros (?) "H". iApply wp_lift_atomic_head_step; eauto.
-  iIntros (σ1 g1 ns κ κs nt) "Hσ1". iMod ("H" $! σ1 with "Hσ1") as "[$ H]"; iModIntro.
+  iIntros (σ1 g1 ns κ κs nt) "Hσ1 Hg1". iMod ("H" $! σ1 with "Hσ1 Hg1") as "[$ H]"; iModIntro.
   iNext; iIntros (v2 σ2 g2 efs Hstep).
-  iMod ("H" $! v2 σ2 g2 efs with "[//]") as "(-> & ? & ?) /=". by iFrame.
+  iMod ("H" $! v2 σ2 g2 efs with "[//]") as "(-> & ? & ? & ?) /=". by iFrame.
 Qed.
 
 Lemma wp_lift_pure_det_head_step_no_fork {s E E' Φ} e1 e2 :
